HeapInsert

HeapInsert.dfy
@@ -1,4 +1,4 @@
-// include "CCPR191-HeapSort-complete-30Dec18.dfy"
+include "CCPR191-HeapSort-complete-30Dec18.dfy"
 
 method {:verify true} Parent(index: nat) returns (p: int) 
 	ensures p == (index - 1) / 2
@@ -10,22 +10,32 @@ function {:verify true} ParentFunc(index: nat) : int
 {
 	(index - 1) / 2
 }
-predicate AncestorIndex(i: nat, j: nat) decreases j-i 
-{ 
-	i == j || (j > 2*i && ((AncestorIndex(2*i+1, j) || AncestorIndex(2*i+2, j))))
-}
-// definition of a heap for the prefix q[..length]
-predicate hp(q: seq<int>, length: nat)
-	requires length <= |q|
+
+function LeftSon(index: nat) : nat 
 {
-	forall i,j :: 0 <= i < length && 0 <= j < length && AncestorIndex(i, j) ==> q[i] >= q[j]
+    2*index+1
 }
-// a partial heap, restricted for elements whose index is in the given set
-predicate ph(q: seq<int>, s: set<nat>)
-	requires (forall e :: e in s ==> e < |q|)
+
+function RightSon(index: nat) : nat 
 {
-	(forall i,j :: i in s && j in s && AncestorIndex(i, j) ==> q[i] >= q[j])
+    2*index+2
 }
+// predicate AncestorIndex(i: nat, j: nat) decreases j-i 
+// { 
+// 	i == j || (j > 2*i && ((AncestorIndex(2*i+1, j) || AncestorIndex(2*i+2, j))))
+// }
+// // definition of a heap for the prefix q[..length]
+// predicate hp(q: seq<int>, length: nat)
+// 	requires length <= |q|
+// {
+// 	forall i,j :: 0 <= i < length && 0 <= j < length && AncestorIndex(i, j) ==> q[i] >= q[j]
+// }
+// // a partial heap, restricted for elements whose index is in the given set
+// predicate ph(q: seq<int>, s: set<nat>)
+// 	requires (forall e :: e in s ==> e < |q|)
+// {
+// 	(forall i,j :: i in s && j in s && AncestorIndex(i, j) ==> q[i] >= q[j])
+// }
 
 predicate phAndHi(q: seq<int>, s: set<nat>, k: nat)
 	requires (forall e :: e in s ==> e < |q|)
@@ -33,22 +43,31 @@ predicate phAndHi(q: seq<int>, s: set<nat>, k: nat)
 	(forall i,j :: i in s && j in s && AncestorIndex(i, j) ==> q[i] >= q[j]) &&
 	forall j :: j in s && AncestorIndex(k, j) ==> q[k] >= q[j]
 }
-// element k is a valid heap element (in the given range) with respect to its ancestors (lower indices)
-predicate lo(q: seq<int>, s: set<nat>, k: nat)
+// // element k is a valid heap element (in the given range) with respect to its ancestors (lower indices)
+predicate loSet(q: seq<int>, s: set<nat>, k: nat)
     requires k < |q| && (forall e :: e in s ==> e < |q|)
 {
 	forall i :: i in s && AncestorIndex(i, k) ==> q[i] >= q[k]
 }
-// element k is a valid heap element (in the given range) with respect to its descendents (higher indices)
-predicate hi(q: seq<int>, s: set<nat>, k: nat)
+// // element k is a valid heap element (in the given range) with respect to its descendents (higher indices)
+predicate hiSet(q: seq<int>, s: set<nat>, k: nat)
 	requires k < |q| && (forall e :: e in s ==> e < |q|)
 {
 	forall j :: j in s && AncestorIndex(k, j) ==> q[k] >= q[j]
 }
 // the suffix q[i..] holds elements in their final (sorted) positions
 
-function IndexSet(start: nat, end: nat, except: nat): set<nat> {
-	 set i: nat | start <= i < end && i != except }
+function IndexSetExcept(start: nat, end: nat, except: nat): set<nat> 
+{
+	set i: nat | start <= i < end && i != except 
+}
+
+lemma Lemma4(a: array<int>, heapsize: nat, x:int, current: nat,parentIndex: int, oldA: multiset<int>)
+	requires WhileInv(a, heapsize, x, current, parentIndex, oldA)
+	requires lo(a[..],0,heapsize,current)
+	ensures hp(a[..], heapsize)
+	ensures oldA == multiset(a[..heapsize])
+{}
 
 method HeapInsert(a: array<int>, heapsize: nat, x: int)
 	requires heapsize < a.Length
@@ -67,7 +86,7 @@ method HeapInsert1a(a: array<int>, heapsize: nat, x: int)
 	requires hp(a[..], heapsize)
     ensures 0 < heapsize + 1 <= a.Length
     ensures multiset(a[..heapsize+1]) == multiset(old(a[..heapsize])+[x])
-    ensures phAndHi(a[..heapsize+1], IndexSet(0, heapsize+1, heapsize), heapsize)
+    ensures phAndHi(a[..heapsize+1], IndexSetExcept(0, heapsize+1, heapsize), heapsize)
     modifies a
 {
     // Assignment
@@ -80,24 +99,25 @@ lemma Lemma1 (a: array<int>, heapsize: nat, x: int)
 	requires hp(a[..], heapsize)
     ensures var newA := a[..heapsize]+[x]; 0 < heapsize + 1 <= |newA| && 
     multiset(newA) == multiset(a[..heapsize]+[x]) && 
-    phAndHi(newA[..heapsize+1], IndexSet(0, heapsize+1, heapsize), heapsize)
+    phAndHi(newA[..heapsize+1], IndexSetExcept(0, heapsize+1, heapsize), heapsize)
 {}
 
 method {:verify true} HeapInsert1b(a: array<int>, heapsize: nat, x: int, ghost oldA: multiset<int>)
     requires 0 < heapsize <= a.Length
     requires multiset(a[..heapsize]) == oldA
-    requires phAndHi(a[..heapsize], IndexSet(0, heapsize, heapsize-1), heapsize-1)
+    requires phAndHi(a[..heapsize], IndexSetExcept(0, heapsize, heapsize-1), heapsize-1)
     ensures hp(a[..], heapsize)
 	ensures multiset(a[..heapsize]) == oldA
 	modifies a
 {
 	var current, parentIndex := InitCurrAndP(a,heapsize, x);
-	Heapify(a, heapsize, x, current, parentIndex, oldA);
+	HeapInsert2(a, heapsize, x, current, parentIndex, oldA);
+    Lemma4(a,heapsize,x,current,parentIndex,oldA);
 }
 
 method {:verify true} InitCurrAndP(a: array<int>, heapsize: nat, x: int) returns(current: nat, parentIndex: int)
     requires 0 < heapsize <= a.Length
-    requires phAndHi(a[..heapsize], IndexSet(0, heapsize, heapsize-1), heapsize-1)
+    requires phAndHi(a[..heapsize], IndexSetExcept(0, heapsize, heapsize-1), heapsize-1)
     ensures current == heapsize - 1 && 0 <= current < a.Length && 
     parentIndex == (current - 1) / 2
 
@@ -108,37 +128,39 @@ method {:verify true} InitCurrAndP(a: array<int>, heapsize: nat, x: int) returns
 
 method {:verify true} InitCurr(a: array<int>, heapsize: nat, x: int) returns(current: nat)
     requires 0 < heapsize <= a.Length
-    requires phAndHi(a[..heapsize], IndexSet(0, heapsize, heapsize-1), heapsize-1)
+    requires phAndHi(a[..heapsize], IndexSetExcept(0, heapsize, heapsize-1), heapsize-1)
     ensures current == heapsize - 1 && 0 <= current < a.Length
-	{
+{
 	LemmaCurr(a, heapsize, x);
 	current := heapsize - 1; 
 }
+
 lemma LemmaCurr (a: array<int>, heapsize: nat, x: int)
 	requires 0 < heapsize <= a.Length
-    requires phAndHi(a[..heapsize], IndexSet(0, heapsize, heapsize-1), heapsize-1)
+    requires phAndHi(a[..heapsize], IndexSetExcept(0, heapsize, heapsize-1), heapsize-1)
 	ensures 0 <= heapsize - 1 < a.Length && heapsize - 1 == heapsize - 1
 {}
 method {:verify true} InitParent(a: array<int>, heapsize: nat, x: int, current: nat) returns(parent: int)
     requires 0 < heapsize <= a.Length
-    requires phAndHi(a[..heapsize], IndexSet(0, heapsize, heapsize-1), heapsize-1)
+    requires phAndHi(a[..heapsize], IndexSetExcept(0, heapsize, heapsize-1), heapsize-1)
     requires current == heapsize - 1 && 0 <= current < a.Length 
 	ensures parent == (current - 1) / 2
 {
 	LemmaParent(a, heapsize, x, current);
 	parent := Parent(current);
 }
+
 lemma LemmaParent (a: array<int>, heapsize: nat, x: int, current: nat)
     requires 0 < heapsize <= a.Length
-    requires phAndHi(a[..heapsize], IndexSet(0, heapsize, heapsize-1), heapsize-1)
+    requires phAndHi(a[..heapsize], IndexSetExcept(0, heapsize, heapsize-1), heapsize-1)
     requires current == heapsize - 1 && 0 <= current < a.Length 
 	ensures ParentFunc(current) == (current - 1) / 2    
 {}
 
-method {:verify true} Heapify(a: array<int>, heapsize: nat, x: int, current0: nat, parentIndex0: int,ghost oldA: multiset<int>)
+method {:verify true} HeapInsert2(a: array<int>, heapsize: nat, x: int, current0: nat, parentIndex0: int,ghost oldA: multiset<int>)
     requires 0 < heapsize <= a.Length
     requires multiset(a[..heapsize]) == oldA
-    requires phAndHi(a[..heapsize], IndexSet(0, heapsize, heapsize-1), current0)
+    requires phAndHi(a[..heapsize], IndexSetExcept(0, heapsize, heapsize-1), current0)
     requires current0 == heapsize - 1 && 0 <= current0 < a.Length && 
     parentIndex0 == (current0 - 1) / 2
     ensures hp(a[..], heapsize)
@@ -146,6 +168,8 @@ method {:verify true} Heapify(a: array<int>, heapsize: nat, x: int, current0: na
 	modifies a
 {
 	var current, parentIndex := current0, parentIndex0; 
+    assert !lo(a[..heapsize], 0, heapsize, current) == Guard1(a, current, parentIndex, heapsize);
+    assert WhileInv(a,  heapsize, x, current, parentIndex, multiset(old(a[..heapsize])));
 	while (Guard1(a, current, parentIndex,heapsize))
 		invariant WhileInv(a, heapsize, x, current, parentIndex, multiset(old(a[..heapsize])))
 		decreases current
@@ -163,12 +187,72 @@ predicate method Guard1(a: array<int>, current: nat, parentIndex: int, heapsize:
     a[current] > a[parentIndex]
 }
 
-predicate WhileInv(a: array<int>, heapsize: nat, x:int, current: nat,parentIndex: int, oldA: multiset<int>)
+predicate WhileInv(a: array<int>, heapsize: nat, x:int, current: nat, parentIndex: int, oldA: multiset<int>)
     reads a
 {
-    parentIndex == (current - 1) / 2 &&
+    0 <= current < heapsize <= a.Length && parentIndex == (current - 1) / 2 &&
 	0 < heapsize <= a.Length && multiset(a[..heapsize]) == oldA &&
-	phAndHi(a[..heapsize], IndexSet(0, heapsize, current),current)
+	phAndHi(a[..heapsize], IndexSetExcept(0, heapsize, current),current)
+}
+
+lemma Lemma3(a: array<int>, heapsize: nat, x: int, current: nat, parentIndex: int, oldA: multiset<int>)
+    requires 0 < heapsize <= a.Length
+    requires multiset(a[..heapsize]) == oldA
+    requires WhileInv(a, heapsize, x, current, parentIndex, oldA)
+    ensures Guard1(a, current, parentIndex, heapsize) == !lo(a[..], 0, heapsize, current)
+{
+    assert !lo(a[..], 0, heapsize, current) == (exists j :: 0 <= j < heapsize && AncestorIndex(j, current) && a[current] > a[j]);
+
+    // Direction 1
+    assert Guard1(a, current, parentIndex, heapsize) ==> (exists j :: 0 <= j < heapsize && AncestorIndex(j, current) && a[current] > a[j]) by {
+        assert 0 < current < heapsize <= a.Length &&  0 <= parentIndex < heapsize <= a.Length && a[current] > a[parentIndex] ==> AncestorIndex(parentIndex, current) ==
+        exists j :: j == parentIndex && AncestorIndex(j, current) && a[current] > a[j];
+    }
+    
+    // Direction 2
+    assert (exists j :: 0 <= j < heapsize && AncestorIndex(j, current) && a[current] > a[j]) ==> Guard1(a, current, parentIndex, heapsize) by {
+
+        // Direction 2.1
+        assert (exists j :: 0 <= j < heapsize && AncestorIndex(j, current) && a[current] > a[j]) ==> 
+        0 < current < heapsize <= a.Length && 0 <= parentIndex < heapsize <= a.Length;
+
+        // Direction 2.2
+        assert (exists j :: 0 <= j < heapsize && AncestorIndex(j, current) && a[current] > a[j]) ==> a[current] > a[parentIndex] by {
+            if (current == 0) {
+                assert (exists j :: 0 <= j < heapsize && AncestorIndex(j, current) && a[current] > a[j]) == Guard1(a, current, parentIndex, heapsize);
+            } else {
+                assert current != 0 ==> 0 < current < heapsize ==> 0 <= parentIndex < heapsize;
+                assert parentIndex == (current - 1) / 2;
+                assert lo(a[..],0,heapsize, parentIndex);
+                assert AncestorIndex(parentIndex, current);
+                forall x | 0 <= x < heapsize && x != current && AncestorIndex(x, current) ensures AncestorIndex(x, parentIndex) {
+                    assert parentIndex <= current;
+                    assert AncestorIndex(x, current);
+                    LemmaLegacy(x, parentIndex, current);
+                }
+            }
+        }
+    }
+}
+
+lemma LemmaLegacy(x: nat, parent: nat, current: nat)
+	requires AncestorIndex(x,current) && AncestorIndex(parent,current)
+	requires parent == (current-1)/2 && x != current
+	ensures AncestorIndex(x,parent)
+	decreases parent-x
+{
+	assert AncestorIndex(x,parent) by {
+		if (x == parent) {
+			assert AncestorIndex(x,parent);
+		} else {
+            // x != parent
+			if (AncestorIndex(LeftSon(x),current)) {
+				LemmaLegacy(LeftSon(x),parent,current);
+			} else {
+				LemmaLegacy(RightSon(x),parent,current);
+			}
+		}
+	}
 }
 
 method {:verify true} LoopBody(a: array<int>, heapsize: nat, x: int, current0: nat, parentIndex0: int, ghost oldA: multiset<int>) returns (current: nat, parentIndex: int)
@@ -189,40 +273,9 @@ method {:verify true} swap (a: array<int>, heapsize: nat, x: int, current: nat, 
     // ensures var newA := a[..parentIndex]+[a[current]]+a[parentIndex+1..current]+[a[parentIndex]]+a[current+1..heapsize];
     && multiset(newA[..heapsize]) == oldA &&
     0 < heapsize <= a.Length &&
-    phAndHi(newA[..heapsize], IndexSet(0, heapsize, parentIndex),parentIndex)
+    phAndHi(newA[..heapsize], IndexSetExcept(0, heapsize, parentIndex),parentIndex)
 	modifies a
 {
-	Lemma2(a ,heapsize,x,current,parentIndex,oldA);
+	// Lemma2(a ,heapsize,x,current,parentIndex,oldA);
 	a[current], a[parentIndex] := a[parentIndex], a[current];
-}
-
-lemma Lemma2(a: array<int>, heapsize: nat, x: int, current: nat, parentIndex: int, oldA: multiset<int>) 
-    requires Guard1(a, current, parentIndex,heapsize)
-    requires WhileInv(a, heapsize, x, current, parentIndex, oldA)
-    ensures var newA := a[..][current := a[parentIndex]][parentIndex := a[current]];
-    && multiset(newA[..heapsize]) == oldA &&
-    0 < heapsize <= a.Length &&
-    phAndHi(newA[..heapsize], IndexSet(0, heapsize, parentIndex),parentIndex)
-{
-    var newA := a[..][current := a[parentIndex]][parentIndex := a[current]];
-    var sParent := IndexSet(0, heapsize, parentIndex);
-    var sCurr := IndexSet(0, heapsize, current);
-    var q,k:= newA[..heapsize], parentIndex;
-    var bliPAndC := IndexSet(0, heapsize, parentIndex) - {current};
-
-    assert ph(a[..heapsize], IndexSet(0, heapsize, current));
-    assert hi(a[..heapsize],IndexSet(0, heapsize, current),parentIndex);
-    assert IndexSet(0, heapsize, current) == IndexSet(0, parentIndex, current) - IndexSet(0, parentIndex, parentIndex)
-    assert lo(a[..heapsize],IndexSet(0, heapsize, current),parentIndex) ==>
-    lo(newA[..heapsize],IndexSet(0, parentIndex, current),current);
-    
-    assert hi(newA[..heapsize],IndexSet(0, heapsize, parentIndex),current);
-
-    // (forall j :: j in sParent && AncestorIndex(current, j) ==> newA[current] >= newA[j]) &&
-    // (forall j :: j in sParent && AncestorIndex(j, current) ==> newA[j] >= newA[current]);
-
-
-    // assert forall j :: j in s && AncestorIndex(k, j) ==> q[k] >= q[j];
-    // assert forall i,j :: i in bliPAndC && j in bliPAndC && AncestorIndex(i, j) ==> q[i] >= q[j];
-    // assert forall i,j :: i in s && j in s && AncestorIndex(i, j) ==> q[i] >= q[j];
 }
